src/program_proof/simplepb/apps/kvee_proof.v
@@ -1,0 +1,126 @@
+From Perennial.program_proof Require Import grove_prelude.
+From Goose.github_com.mit_pdos.gokv.simplepb.apps Require Import kvee.
+From Perennial.program_proof Require Import marshal_stateless_proof.
+From iris.base_logic Require Import ghost_map.
+From Perennial.goose_lang Require Import crash_borrow.
+From Perennial.program_proof.simplepb.simplelog Require Import proof.
+From Perennial.program_proof.simplepb Require Import pb_definitions.
+From Perennial.program_proof.simplepb Require Import pb_apply_proof clerk_proof.
+From Perennial.program_proof.grove_shared Require Import erpc_lib.
+From Perennial.program_proof Require Import map_marshal_proof.
+From Perennial.program_proof Require Import map_marshal_proof.
+From iris.algebra Require Import dfrac_agree mono_list.
+
+From Perennial.program_proof.simplepb.apps Require Import eesm_proof kv_proof.
+
+Section global_proof.
+
+Context `{!heapGS Σ}.
+Definition eekv_record := (ee_record (low_record:=kv_record)).
+Context `{!simplelogG (sm_record:=eekv_record) Σ}.
+
+Lemma wp_Start fname (host:chan) γsys γsrv data :
+  {{{
+      "#Hhost" ∷ is_pb_host host γsys γsrv ∗
+      "#Hinv" ∷ sys_inv γsys ∗
+      "Hfile_ctx" ∷ crash_borrow (fname f↦ data ∗ file_crash (own_Server_ghost γsys γsrv) data)
+                    (|C={⊤}=> ∃ data', fname f↦ data' ∗ ▷ file_crash (own_Server_ghost γsys γsrv) data')
+  }}}
+    Start #(host:u64) #(LitString fname)
+  {{{
+        RET #(); True
+  }}}
+.
+Proof.
+  iIntros (Φ) "Hpre HΦ".
+  iNamed "Hpre".
+  wp_call.
+  wp_apply (wp_MakeKVStateMachine).
+  iIntros (??) "[#His1 Hown]".
+  wp_apply (wp_MakeEEKVStateMachine with "[Hown]").
+  {
+    iFrame "His1".
+    iFrame.
+  }
+  iIntros (??) "[#His2 Hown]".
+  wp_apply (wp_MakePbServer (sm_record:=eekv_record) with "Hinv [$His2 $Hown $Hfile_ctx]").
+  iIntros (?) "His".
+  wp_pures.
+  wp_apply (pb_start_proof.wp_Server__Serve with "[$]").
+  wp_pures.
+  by iApply "HΦ".
+Qed.
+
+Notation own_oplog := (own_oplog (low_record:=kv_record)).
+
+Context `{!kv64G Σ}.
+Context `{!erpcG Σ (list u8)}.
+Definition eekv_inv γ γkv : iProp Σ :=
+  inv stateN (∃ ops, own_oplog γ ops ∗ own_kvs γkv ops).
+
+Definition own_Clerk ck γkv : iProp Σ :=
+  ∃ (eeCk:loc) γlog,
+    "Hcl" ∷ ck ↦[kvee.Clerk :: "cl"] #eeCk ∗
+    "#Hkvinv" ∷ kv_inv γlog γkv ∗
+    "Hownck" ∷ eesm_proof.own_Clerk eeCk γlog
+.
+
+Lemma wp_Clerk__Put ck γkv key val_sl value Φ:
+  own_Clerk ck γkv -∗
+  is_slice_small val_sl byteT 1 value -∗
+  (|={⊤∖↑pbN∖↑eeN,↑stateN}=> ∃ old_value, kv_ptsto γkv key old_value ∗
+    (kv_ptsto γkv key (value) ={↑stateN,⊤∖↑pbN∖↑eeN}=∗
+    (own_Clerk ck γkv -∗ Φ #()))) -∗
+  WP Clerk__Put #ck #key (slice_val val_sl) {{ Φ }}.
+Proof.
+  iIntros "Hck Hval_sl Hupd".
+  wp_lam.
+  wp_pures.
+  wp_apply (wp_allocStruct).
+  { Transparent slice.T. repeat econstructor. Opaque slice.T. }
+  iIntros (args) "Hargs".
+  iDestruct (struct_fields_split with "Hargs") as "HH".
+  iNamed "HH".
+  wp_pures.
+  iNamed "Hck".
+  wp_apply (wp_EncodePutArgs with "[$Key $Val $Hval_sl]").
+  iIntros (putEncoded put_sl) "[%Henc Henc_sl]".
+  wp_loadField.
+  wp_apply (wp_Clerk__ApplyExactlyOnce with "Hownck Henc_sl").
+  { done. }
+
+  (* make this a separate lemma? *)
+  iMod "Hupd".
+
+  iInv "Hkvinv" as ">Hown" "Hclose".
+  replace (↑_∖_) with (∅:coPset); last set_solver.
+  iModIntro.
+
+  iDestruct "Hown" as (?) "[Hlog Hkvs]".
+  iDestruct ("Hupd") as (?) "[Hkvptsto Hkvclose]".
+  iExists _; iFrame "Hlog".
+  iIntros "Hlog".
+
+  iMod (ghost_map_update (value) with "Hkvs Hkvptsto") as "[Hkvs Hkvptsto]".
+
+  iMod ("Hclose" with "[Hlog Hkvs]") as "_".
+  {
+    iExists _; iFrame.
+    iNext.
+    unfold own_kvs.
+    unfold compute_state.
+    rewrite foldl_snoc.
+    simpl.
+    iFrame.
+  }
+  iMod ("Hkvclose" with "Hkvptsto") as "HH".
+  iModIntro.
+  iIntros (?) "Hsl Hck".
+  wp_pures.
+  iApply "HH".
+  iModIntro.
+  repeat iExists _.
+  iFrame "∗#".
+Qed.
+
+End global_proof.
